# baseURI: http://www.w3.org/ns/ssn-ext
# imports: http://www.w3.org/ns/ssn/

@prefix dcterms: <http://purl.org/dc/terms/> .
@prefix owl: <http://www.w3.org/2002/07/owl#> .
@prefix rdf: <http://www.w3.org/1999/02/22-rdf-syntax-ns#> .
@prefix rdfs: <http://www.w3.org/2000/01/rdf-schema#> .
@prefix schema: <http://schema.org/> .
@prefix skos: <http://www.w3.org/2004/02/skos/core#> .
@prefix sosa: <http://www.w3.org/ns/sosa/> .
@prefix ssn: <http://www.w3.org/ns/ssn/> .
@prefix ssn-ext: <http://www.w3.org/ns/ssn-ext/> .
@prefix time: <http://www.w3.org/2006/time#> .
@prefix xsd: <http://www.w3.org/2001/XMLSchema#> .

sosa:Observation
  rdfs:comment """*** TODO ***
Need to add SPIN rules to populate missing values by copying them down from a parent collection
e.g. something like (for each of hasFeatureOfInterest, madeBySensor, observedProperty, phenomenonTime, usedProcedure, resultTime
 
CONSTRUCT { ?o sosa:hasFeatureOfInterest ?foi }
WHERE{
  ?oc sosa:hasMemberObservation ?o . 
  ?oc sosa:hasFeatureOfInterest ?foi . 
  NOT EXISTS { ?o sosa:hasFeatureOfInterest ?x }
}

... but don't quite grok the SPIN/SPARQL syntax yet""" ;
  rdfs:subClassOf [
      rdf:type owl:Restriction ;
      owl:minCardinality "1"^^xsd:nonNegativeInteger ;
      owl:onProperty sosa:hasUltimateFeatureOfInterest ;
    ] ;
.
sosa:ObservationCollection
  rdf:type owl:Class ;
  rdfs:comment "Collection of observations, typically with one or more property common across all members" ;
  rdfs:label "Collection of observations" ;
  rdfs:subClassOf [
      rdf:type owl:Restriction ;
      owl:allValuesFrom xsd:dateTime ;
      owl:onProperty sosa:resultTime ;
    ] ;
  rdfs:subClassOf [
      rdf:type owl:Restriction ;
      owl:allValuesFrom time:TemporalEntity ;
      owl:onProperty sosa:phenomenonTime ;
    ] ;
  rdfs:subClassOf [
      rdf:type owl:Restriction ;
      owl:allValuesFrom sosa:FeatureOfInterest ;
      owl:onProperty sosa:hasFeatureOfInterest ;
    ] ;
  rdfs:subClassOf [
      rdf:type owl:Restriction ;
      owl:allValuesFrom sosa:FeatureOfInterest ;
      owl:onProperty sosa:hasUltimateFeatureOfInterest ;
    ] ;
  rdfs:subClassOf [
      rdf:type owl:Restriction ;
      owl:allValuesFrom sosa:ObservableProperty ;
      owl:onProperty sosa:observedProperty ;
    ] ;
  rdfs:subClassOf [
      rdf:type owl:Restriction ;
      owl:allValuesFrom sosa:Procedure ;
      owl:onProperty sosa:usedProcedure ;
    ] ;
  rdfs:subClassOf [
      rdf:type owl:Restriction ;
      owl:allValuesFrom sosa:Sensor ;
      owl:onProperty sosa:madeBySensor ;
    ] ;
  rdfs:subClassOf [
      rdf:type owl:Restriction ;
      owl:minCardinality "1"^^xsd:nonNegativeInteger ;
      owl:onProperty sosa:hasMemberObservation ;
    ] ;
.
sosa:Sampling
  rdfs:subClassOf [
      rdf:type owl:Restriction ;
      owl:minCardinality "1"^^xsd:nonNegativeInteger ;
      owl:onProperty sosa:hasUltimateFeatureOfInterest ;
    ] ;
.
sosa:hasFeatureOfInterest
  schema:domainIncludes sosa:ObservationCollection ;
.
sosa:hasMemberObservation
  rdf:type owl:ObjectProperty ;
  schema:domainIncludes sosa:ObservationCollection ;
  schema:rangeIncludes sosa:Observation ;
  rdfs:comment "Link to a member of a collection of observations that share the same value for one or more of the characteristic properties" ;
  rdfs:domain sosa:ObservationCollection ;
  rdfs:label "member observation" ;
  rdfs:range sosa:Observation ;
  rdfs:subPropertyOf rdfs:member ;
.
sosa:hasUltimateFeatureOfInterest
  rdf:type owl:ObjectProperty ;
  schema:domainIncludes sosa:Actuation ;
  schema:domainIncludes sosa:Observation ;
  schema:domainIncludes sosa:Sampling ;
  schema:rangeIncludes sosa:FeatureOfInterest ;
  rdfs:comment "link to the ultimate feature of interest of an observation or act of sampling. This is useful when the proximate feature of interest is a sample of the ultimate feature of interest, directly or trasntitively." ;
  rdfs:label "has ultimate feature of interest" ;
.
sosa:madeBySensor
  schema:domainIncludes sosa:ObservationCollection ;
.
sosa:observedProperty
  schema:domainIncludes sosa:ObservationCollection ;
.
sosa:phenomenonTime
  schema:domainIncludes sosa:ObservationCollection ;
.
sosa:resultTime
  schema:domainIncludes sosa:ObservationCollection ;
.
sosa:usedProcedure
  schema:domainIncludes sosa:ObservationCollection ;
.
<http://www.w3.org/ns/ssn-ext>
  rdf:type owl:Ontology ;
  dcterms:created "2018-03-08" ;
  dcterms:creator "<http://orcid.org/0000-0002-3884-3420>" ;
  rdfs:comment "Some extensions to the SSN Ontology" ;
  rdfs:label "SSN extensions" ;
  owl:imports ssn: ;
.
