<?xml version="1.0"?>
<rdf:RDF
    xmlns:rdf="http://www.w3.org/1999/02/22-rdf-syntax-ns#"
    xmlns:schema="http://schema.org/"
    xmlns:rdfs="http://www.w3.org/2000/01/rdf-schema#"
    xmlns:ssn-ext="http://www.w3.org/ns/ssn/ext/"
    xmlns:dcterms="http://purl.org/dc/terms/"
    xmlns:ex="http://example.org/"
    xmlns:time="http://www.w3.org/2006/time#"
    xmlns:owl="http://www.w3.org/2002/07/owl#"
    xmlns:sosa="http://www.w3.org/ns/sosa/"
    xmlns:skos="http://www.w3.org/2004/02/skos/core#"
    xmlns:sh="http://www.w3.org/ns/shacl#"
    xmlns:ssn="http://www.w3.org/ns/ssn/"
    xmlns:xsd="http://www.w3.org/2001/XMLSchema#"
  xml:base="http://www.w3.org/ns/ssn/ext">
  <owl:Ontology rdf:about="">
    <dcterms:description>Some extensions to the SSN Ontology, to support&#xD;
&#xD;
1. discovery and use of observation and sample data through links to an ultimate feature-of-interest, or sample&#xD;
2. observations are  made as part of a set or collection, in which one or more of the observation properties - hasFeatureOfInterest, observedProperty, madeBySensor, usedProcedure, phenomenonTime, resultTime - are shared by all members of the collection. &#xD;
&#xD;
These extensions to the SSN Ontology are packaged in a separate RDF graph to enable loading and use if required. </dcterms:description>
    <dcterms:rights>Copyright 2019 W3C/OGC.</dcterms:rights>
    <rdfs:comment>The classes, properties, and axioms in this RDF graph are described in https://www.w3.org/TR/vocab-ssn-ext/&#xD;
&#xD;
Their status is non-normative, and SSN applications are not required to recognize or support them. </rdfs:comment>
    <dcterms:created rdf:datatype="http://www.w3.org/2001/XMLSchema#date"
    >2018-03-08</dcterms:created>
    <dcterms:license rdf:resource="http://www.opengeospatial.org/ogc/Software"/>
    <dcterms:modified rdf:datatype="http://www.w3.org/2001/XMLSchema#date"
    >2019-12-24</dcterms:modified>
    <rdfs:label>SSN extensions</rdfs:label>
    <dcterms:license rdf:resource="http://www.w3.org/Consortium/Legal/2015/copyright-software-and-document"/>
    <dcterms:creator rdf:resource="http://orcid.org/0000-0002-3884-3420"/>
    <owl:imports rdf:resource="http://www.w3.org/ns/ssn/"/>
    <dcterms:title xml:lang="en">Extensions to the SSN Ontology</dcterms:title>
  </owl:Ontology>
  <owl:Class rdf:about="http://www.w3.org/ns/sosa/ObservationCollection">
    <rdfs:subClassOf>
      <owl:Restriction>
        <owl:onProperty>
          <rdf:Description rdf:about="http://www.w3.org/ns/sosa/hasFeatureOfInterest">
            <schema:domainIncludes rdf:resource="http://www.w3.org/ns/sosa/ObservationCollection"/>
          </rdf:Description>
        </owl:onProperty>
        <owl:maxCardinality rdf:datatype="http://www.w3.org/2001/XMLSchema#nonNegativeInteger"
        >1</owl:maxCardinality>
      </owl:Restriction>
    </rdfs:subClassOf>
    <rdfs:subClassOf>
      <owl:Restriction>
        <owl:onProperty>
          <rdf:Description rdf:about="http://www.w3.org/ns/sosa/observedProperty">
            <schema:domainIncludes rdf:resource="http://www.w3.org/ns/sosa/ObservationCollection"/>
          </rdf:Description>
        </owl:onProperty>
        <owl:allValuesFrom rdf:resource="http://www.w3.org/ns/sosa/ObservableProperty"/>
      </owl:Restriction>
    </rdfs:subClassOf>
    <rdfs:subClassOf>
      <owl:Restriction>
        <owl:onProperty rdf:resource="http://www.w3.org/ns/ssn/wasOriginatedBy"/>
        <owl:allValuesFrom rdf:resource="http://www.w3.org/ns/ssn/Stimulus"/>
      </owl:Restriction>
    </rdfs:subClassOf>
    <rdfs:subClassOf>
      <owl:Restriction>
        <owl:onProperty>
          <rdf:Description rdf:about="http://www.w3.org/ns/sosa/madeBySensor">
            <schema:domainIncludes rdf:resource="http://www.w3.org/ns/sosa/ObservationCollection"/>
          </rdf:Description>
        </owl:onProperty>
        <owl:maxCardinality rdf:datatype="http://www.w3.org/2001/XMLSchema#nonNegativeInteger"
        >1</owl:maxCardinality>
      </owl:Restriction>
    </rdfs:subClassOf>
    <rdfs:subClassOf>
      <owl:Restriction>
        <owl:onProperty>
          <owl:ObjectProperty rdf:about="http://www.w3.org/ns/sosa/hasUltimateFeatureOfInterest"/>
        </owl:onProperty>
        <owl:allValuesFrom rdf:resource="http://www.w3.org/ns/sosa/FeatureOfInterest"/>
      </owl:Restriction>
    </rdfs:subClassOf>
    <rdfs:subClassOf>
      <owl:Restriction>
        <owl:onProperty>
          <rdf:Description rdf:about="http://www.w3.org/ns/sosa/usedProcedure">
            <schema:domainIncludes rdf:resource="http://www.w3.org/ns/sosa/ObservationCollection"/>
          </rdf:Description>
        </owl:onProperty>
        <owl:maxCardinality rdf:datatype="http://www.w3.org/2001/XMLSchema#nonNegativeInteger"
        >1</owl:maxCardinality>
      </owl:Restriction>
    </rdfs:subClassOf>
    <rdfs:label>Collection of observations</rdfs:label>
    <rdfs:subClassOf>
      <owl:Restriction>
        <owl:onProperty>
          <rdf:Description rdf:about="http://www.w3.org/ns/sosa/resultTime">
            <schema:domainIncludes rdf:resource="http://www.w3.org/ns/sosa/ObservationCollection"/>
          </rdf:Description>
        </owl:onProperty>
        <owl:maxCardinality rdf:datatype="http://www.w3.org/2001/XMLSchema#nonNegativeInteger"
        >1</owl:maxCardinality>
      </owl:Restriction>
    </rdfs:subClassOf>
    <rdfs:subClassOf>
      <owl:Restriction>
        <owl:onProperty>
          <owl:ObjectProperty rdf:about="http://www.w3.org/ns/sosa/hasMember"/>
        </owl:onProperty>
        <owl:minCardinality rdf:datatype="http://www.w3.org/2001/XMLSchema#nonNegativeInteger"
        >1</owl:minCardinality>
      </owl:Restriction>
    </rdfs:subClassOf>
    <rdfs:subClassOf>
      <owl:Restriction>
        <owl:onProperty rdf:resource="http://www.w3.org/ns/sosa/hasFeatureOfInterest"/>
        <owl:allValuesFrom rdf:resource="http://www.w3.org/ns/sosa/FeatureOfInterest"/>
      </owl:Restriction>
    </rdfs:subClassOf>
    <rdfs:subClassOf>
      <owl:Restriction>
        <owl:onProperty rdf:resource="http://www.w3.org/ns/sosa/madeBySensor"/>
        <owl:allValuesFrom rdf:resource="http://www.w3.org/ns/sosa/Sensor"/>
      </owl:Restriction>
    </rdfs:subClassOf>
    <rdfs:subClassOf>
      <owl:Restriction>
        <owl:onProperty rdf:resource="http://www.w3.org/ns/sosa/observedProperty"/>
        <owl:maxCardinality rdf:datatype="http://www.w3.org/2001/XMLSchema#nonNegativeInteger"
        >1</owl:maxCardinality>
      </owl:Restriction>
    </rdfs:subClassOf>
    <rdfs:subClassOf>
      <owl:Restriction>
        <owl:onProperty rdf:resource="http://www.w3.org/ns/sosa/usedProcedure"/>
        <owl:allValuesFrom rdf:resource="http://www.w3.org/ns/sosa/Procedure"/>
      </owl:Restriction>
    </rdfs:subClassOf>
    <rdfs:subClassOf>
      <owl:Restriction>
        <owl:onProperty>
          <rdf:Description rdf:about="http://www.w3.org/ns/sosa/phenomenonTime">
            <schema:domainIncludes rdf:resource="http://www.w3.org/ns/sosa/ObservationCollection"/>
          </rdf:Description>
        </owl:onProperty>
        <owl:maxCardinality rdf:datatype="http://www.w3.org/2001/XMLSchema#nonNegativeInteger"
        >1</owl:maxCardinality>
      </owl:Restriction>
    </rdfs:subClassOf>
    <rdfs:comment>Collection of observations, typically with one or more property shared by all of its members</rdfs:comment>
    <rdfs:subClassOf>
      <owl:Restriction>
        <owl:onProperty>
          <owl:ObjectProperty rdf:about="http://www.w3.org/ns/sosa/hasUltimateFeatureOfInterest"/>
        </owl:onProperty>
        <owl:maxCardinality rdf:datatype="http://www.w3.org/2001/XMLSchema#nonNegativeInteger"
        >1</owl:maxCardinality>
      </owl:Restriction>
    </rdfs:subClassOf>
  </owl:Class>
  <owl:ObjectProperty rdf:about="http://www.w3.org/ns/sosa/hasMember">
    <rdfs:subPropertyOf rdf:resource="http://www.w3.org/2000/01/rdf-schema#member"/>
    <rdfs:range>
      <owl:Class>
        <owl:unionOf rdf:parseType="Collection">
          <rdf:Description rdf:about="http://www.w3.org/ns/sosa/Observation">
            <rdfs:subClassOf>
              <owl:Restriction>
                <owl:onProperty>
                  <owl:ObjectProperty rdf:about="http://www.w3.org/ns/sosa/hasUltimateFeatureOfInterest"/>
                </owl:onProperty>
                <owl:minCardinality rdf:datatype="http://www.w3.org/2001/XMLSchema#nonNegativeInteger"
                >1</owl:minCardinality>
              </owl:Restriction>
            </rdfs:subClassOf>
            <rdfs:comment>If values are not provided for the following Observation properties, they may be provided by the ObservationCollection of which it is a member:&#xD;
- hasFeatureOfInterest&#xD;
- hasUltimateFeatureOfInterest&#xD;
- madeBySensor&#xD;
- observedProperty&#xD;
- phenomenonTime&#xD;
- resultTime&#xD;
- usedProcedure</rdfs:comment>
          </rdf:Description>
          <owl:Class rdf:about="http://www.w3.org/ns/sosa/ObservationCollection"/>
        </owl:unionOf>
      </owl:Class>
    </rdfs:range>
    <rdfs:label>member observation</rdfs:label>
    <rdfs:domain rdf:resource="http://www.w3.org/ns/sosa/ObservationCollection"/>
    <rdfs:comment>Link to a member within a collection of (observations) or (collections of observations) that share the same value for one or more of the characteristic properties</rdfs:comment>
    <schema:rangeIncludes rdf:resource="http://www.w3.org/ns/sosa/ObservationCollection"/>
    <schema:rangeIncludes rdf:resource="http://www.w3.org/ns/sosa/Observation"/>
    <schema:domainIncludes rdf:resource="http://www.w3.org/ns/sosa/ObservationCollection"/>
  </owl:ObjectProperty>
  <owl:ObjectProperty rdf:about="http://www.w3.org/ns/sosa/hasUltimateFeatureOfInterest">
    <rdfs:range rdf:resource="http://www.w3.org/ns/sosa/FeatureOfInterest"/>
    <schema:domainIncludes rdf:resource="http://www.w3.org/ns/sosa/Observation"/>
    <rdfs:label>has ultimate feature of interest</rdfs:label>
    <rdfs:domain>
      <owl:Class>
        <owl:unionOf rdf:parseType="Collection">
          <rdf:Description rdf:about="http://www.w3.org/ns/sosa/Observation"/>
          <rdf:Description rdf:about="http://www.w3.org/ns/sosa/Sampling">
            <rdfs:subClassOf>
              <owl:Restriction>
                <owl:onProperty rdf:resource="http://www.w3.org/ns/sosa/hasUltimateFeatureOfInterest"/>
                <owl:minCardinality rdf:datatype="http://www.w3.org/2001/XMLSchema#nonNegativeInteger"
                >1</owl:minCardinality>
              </owl:Restriction>
            </rdfs:subClassOf>
          </rdf:Description>
          <rdf:Description rdf:about="http://www.w3.org/ns/sosa/Actuation">
            <rdfs:subClassOf>
              <owl:Restriction>
                <owl:onProperty rdf:resource="http://www.w3.org/ns/sosa/hasUltimateFeatureOfInterest"/>
                <owl:minCardinality rdf:datatype="http://www.w3.org/2001/XMLSchema#nonNegativeInteger"
                >1</owl:minCardinality>
              </owl:Restriction>
            </rdfs:subClassOf>
          </rdf:Description>
        </owl:unionOf>
      </owl:Class>
    </rdfs:domain>
    <rdfs:comment>should match a property chain something like this but with sosa:isSampleOf*&#xD;
      owl:propertyChainAxiom ( sosa:hasFeatureOfInterest sosa:isSampleOf )</rdfs:comment>
    <schema:domainIncludes rdf:resource="http://www.w3.org/ns/sosa/Sampling"/>
    <rdfs:comment>link to the ultimate feature of interest of an observation or act of sampling. This is useful when the proximate feature of interest is a sample of the ultimate feature of interest, directly or trasntitively.</rdfs:comment>
    <schema:rangeIncludes rdf:resource="http://www.w3.org/ns/sosa/FeatureOfInterest"/>
    <schema:domainIncludes rdf:resource="http://www.w3.org/ns/sosa/Actuation"/>
  </owl:ObjectProperty>
  <owl:ObjectProperty rdf:about="http://www.w3.org/ns/sosa/hasOriginalSample">
    <rdfs:range>
      <rdf:Description rdf:about="http://www.w3.org/ns/sosa/Sample">
        <rdfs:subClassOf>
          <owl:Restriction>
            <owl:onProperty>
              <owl:ObjectProperty rdf:about="http://www.w3.org/ns/sosa/hasSampledFeature"/>
            </owl:onProperty>
            <owl:minCardinality rdf:datatype="http://www.w3.org/2001/XMLSchema#nonNegativeInteger"
            >1</owl:minCardinality>
          </owl:Restriction>
        </rdfs:subClassOf>
        <rdfs:subClassOf>
          <owl:Restriction>
            <owl:onProperty rdf:resource="http://www.w3.org/ns/sosa/hasOriginalSample"/>
            <owl:maxCardinality rdf:datatype="http://www.w3.org/2001/XMLSchema#nonNegativeInteger"
            >1</owl:maxCardinality>
          </owl:Restriction>
        </rdfs:subClassOf>
      </rdf:Description>
    </rdfs:range>
    <rdfs:label>has original sample</rdfs:label>
    <rdfs:domain rdf:resource="http://www.w3.org/ns/sosa/Sample"/>
    <rdfs:comment>link to the original sample that is related to the context sample through a chain of isSampleOf relations</rdfs:comment>
    <schema:rangeIncludes rdf:resource="http://www.w3.org/ns/sosa/Sample"/>
    <schema:domainIncludes rdf:resource="http://www.w3.org/ns/sosa/Sample"/>
  </owl:ObjectProperty>
  <owl:ObjectProperty rdf:about="http://www.w3.org/ns/sosa/hasSampledFeature">
    <rdfs:range rdf:resource="http://www.w3.org/ns/sosa/FeatureOfInterest"/>
    <rdfs:label>is ultimate sample of</rdfs:label>
    <rdfs:domain rdf:resource="http://www.w3.org/ns/sosa/Sample"/>
    <rdfs:comment>link to the ultimate feature of interest of the context sample - i.e. the end of a chain of isSampleOf relations</rdfs:comment>
    <schema:rangeIncludes rdf:resource="http://www.w3.org/ns/sosa/FeatureOfInterest"/>
    <schema:domainIncludes rdf:resource="http://www.w3.org/ns/sosa/Sample"/>
  </owl:ObjectProperty>
</rdf:RDF>

