# baseURI: https://www.w3.org/ns/sosa
# imports: http://schema.org

@prefix dc: <http://purl.org/dc/elements/1.1/> .
@prefix ns: <http://creativecommons.org/ns#> .
@prefix owl: <http://www.w3.org/2002/07/owl#> .
@prefix rdf: <http://www.w3.org/1999/02/22-rdf-syntax-ns#> .
@prefix rdfs: <http://www.w3.org/2000/01/rdf-schema#> .
@prefix schema: <http://schema.org/> .
@prefix sosa-core: <https://www.w3.org/ns/sosa#> .
@prefix terms: <http://purl.org/dc/terms/> .
@prefix xhtm: <http://www.w3.org/1999/xhtml> .
@prefix xsd: <http://www.w3.org/2001/XMLSchema#> .

ns:license
  rdf:type owl:AnnotationProperty ;
.
dc:creator
  rdf:type owl:AnnotationProperty ;
.
dc:date
  rdf:type owl:AnnotationProperty ;
.
dc:identifier
  rdf:type owl:AnnotationProperty ;
.
dc:rights
  rdf:type owl:AnnotationProperty ;
.
dc:source
  rdf:type owl:AnnotationProperty ;
.
dc:title
  rdf:type owl:AnnotationProperty ;
.
terms:created
  rdf:type owl:AnnotationProperty ;
.
terms:modified
  rdf:type owl:AnnotationProperty ;
.
schema:domainIncludes
  rdf:type owl:AnnotationProperty ;
.
schema:rangeIncludes
  rdf:type owl:AnnotationProperty ;
.
rdfs:comment
  rdf:type owl:AnnotationProperty ;
.
rdfs:isDefinedBy
  rdf:type owl:AnnotationProperty ;
.
rdfs:label
  rdf:type owl:AnnotationProperty ;
.
rdfs:seeAlso
  rdf:type owl:AnnotationProperty ;
.
owl:topObjectProperty
  rdf:type owl:ObjectProperty ;
.
<https://www.w3.org/ns/sosa>
  rdf:type owl:Ontology ;
  rdfs:comment "Sensing, Observing, Sampling, and Actuating (SOSA) Core Ontology "^^xsd:string ;
  rdfs:comment "This ontology is based on the SSN Ontology by the W3C Semantic Sensor Networks Incubator Group (SSN-XG), together with considerations from the W3C/OGC Spatial Data on the Web Working Group."^^xsd:string ;
  rdfs:comment "This version is based on the horizontal/vertical modularization proposed by Jano for the W3C/OGC Spatial Data on the Web Working Group: https://www.w3.org/2015/spatial/wiki/SOSA_Ontology and https://www.w3.org/2015/spatial/wiki/SSN_core_modules"^^xsd:string ;
  rdfs:label "Sensing, Observing, Sampling, and Actuating"^^xsd:string ;
  owl:imports <http://schema.org> ;
.
sosa-core:Activity
  rdf:type rdfs:Class ;
  rdfs:comment "An action or event during which a Procedure is used."@en ;
  rdfs:label "Activity"@en ;
  rdfs:subClassOf owl:Thing ;
.
sosa-core:ActuatingProcedure
  rdf:type owl:Class ;
  rdfs:comment "When used, an ActuationProcedure can cause a change in the state of the world."@en ;
  rdfs:label "Actuating Procedure"@en ;
  rdfs:subClassOf sosa-core:Procedure ;
.
sosa-core:Actuation
  rdf:type rdfs:Class ;
  rdfs:comment "An Activity that uses an ActuatingProcedure to cause a change in the state of the world, for example by moving something, heating it up, turning it on."@en ;
  rdfs:label "Actuation"@en ;
  rdfs:subClassOf sosa-core:Activity ;
.
sosa-core:Actuator
  rdf:type owl:Class ;
  rdfs:comment "A Device that is used by, or implements, an Actuating Procedure."@en ;
  rdfs:label "Actuator"@en ;
  rdfs:subClassOf sosa-core:Device ;
.
sosa-core:Device
  rdf:type owl:Class ;
  rdfs:comment "A physical object involved in a Procedure that observes, samples, or changes the state of the world."@en ;
  rdfs:label "Device"@en ;
  rdfs:subClassOf owl:Thing ;
.
sosa-core:ObservableProperty
  rdf:type owl:Class ;
  rdfs:comment "An observable Quality of a thing; typically a FeatureOfInterest."@en ;
  rdfs:label "Observable Property"@en ;
.
sosa-core:Observation
  rdf:type owl:Class ;
  rdfs:comment "An Observation is an Activity in which a Sensing method or ObservationProcedure has been used to estimate or calculate a value of a Property of a FeatureOfInterest. Links to an Observer or Sensor to describe what made the Observation and how; links to FeatureOfInterest detail what was observed; the Result is the output."@en ;
  rdfs:label "Observation"@en ;
  rdfs:subClassOf sosa-core:Activity ;
.
sosa-core:Observer
  rdf:type owl:Class ;
  rdfs:comment "Device or agent involved in, or implementing, an ObservingProcedure."@en ;
  rdfs:label "Observer"@en ;
  rdfs:subClassOf sosa-core:Device ;
.
sosa-core:ObservingProcedure
  rdf:type owl:Class ;
  rdfs:comment "Procedure used to make an estimate of the value of a quality of a feature. Input may be a sensor stimulus, or the output from one or more previous activities."@en ;
  rdfs:label "Observing procedure"@en ;
  rdfs:subClassOf sosa-core:Procedure ;
.
sosa-core:Platform
  rdf:type owl:Class ;
  rdfs:comment "A Device or agent on which other Devices are mounted or hosted. Maybe stationary, moving, or portable. Examples include: station, buoy, ship, planes, satellite, balloon, cell-phone, table, tractor, automobile."@en ;
  rdfs:label "Platform"@en ;
  rdfs:subClassOf sosa-core:Device ;
.
sosa-core:Procedure
  rdf:type owl:Class ;
  rdfs:comment "Software, protocol, computational method, algorithm or plan responsible for generating an observation Result, or taking a Sample, or making a change to the state of the world. A Procedure is re-usable, and might be involved in many observations, samplings, or actuations."@en ;
  rdfs:label "Procedure"@en ;
.
sosa-core:Sampling
  rdf:type rdfs:Class ;
  rdfs:comment "An Activity that uses a SamplingProcedure to obtain or define a SamplingFeature (sample), such as a subset, specimen, cross-section, transect etc."@en ;
  rdfs:label "Sampling"@en ;
  rdfs:subClassOf sosa-core:Activity ;
.
sosa-core:SamplingDevice
  rdf:type owl:Class ;
  rdfs:comment "Device used to obtain a sample"@en ;
  rdfs:label "Sampling device"@en ;
  rdfs:subClassOf sosa-core:Device ;
.
sosa-core:SamplingFeature
  rdf:type owl:Class ;
  rdfs:comment "Feature on which observations may be made, which is intended to be representative of a FeatureOfInterest that is not fully accessible."@en ;
  rdfs:comment """Sampling features are artifacts of an observational strategy, and have no significant function outside of their role in the observation process. The physical characteristics of the features themselves are of little interest, except perhaps to the manager of a sampling campaign.

EXAMPLE A “station” is essentially an identifiable locality where a sensor system or procedure may be deployed and an observation made. In the context of the observation model, it connotes the “world in the vicinity of the station”, so the observed properties relate to the physical medium at the station, and not to any physical artifact such as a mooring, buoy, benchmark, monument, well, etc.

NOTE A transient sampling feature, such as a ships-track or flight-line, might be identified and described, but is unlikely to be revisited exactly.

A sampling feature is intended to sample some feature-of-interest in an application domain, so there is an expectation of at least one sampledFeature property. However, in some cases the identity, and even the exact type, of the sampled feature may not be known when observations are made using the sampling features."""@en ;
  rdfs:label "Sample"@en ;
  rdfs:label "Sampling Feature"@en ;
.
sosa-core:SamplingProcedure
  rdf:type owl:Class ;
  rdfs:comment "A Procedure of sampling, i.e., a description of the sampling process a sampling device can execute."@en ;
  rdfs:label "Sampling Procedure"@en ;
  rdfs:subClassOf sosa-core:Procedure ;
.
sosa-core:Sensing
  rdf:type owl:Class ;
  rdfs:comment "Sensing is an Activity in which a SensingProcedure has been used to estimate or calculate a value of a Property of a FeatureOfInterest. Links to a or Sensor to describe what performed the Sensing and how; links to FeatureOfInterest detail what was observed; the Result is the output."@en ;
  rdfs:label "Sensing"@en ;
  rdfs:subClassOf sosa-core:Observation ;
.
sosa-core:SensingProcedure
  rdf:type owl:Class ;
  rdfs:comment "A Procedure of sensing, i.e. a description of a procedure that uses or is implemented by a SensingDevice."@en ;
  rdfs:label "Sensing Procedure"@en ;
  rdfs:subClassOf sosa-core:ObservingProcedure ;
.
sosa-core:Sensor
  rdf:type owl:Class ;
  rdfs:comment "Device or agent involved in, or implementing, a SensingProcedure. Responds to a stimulus and generates a result."@en ;
  rdfs:label "Sensor"@en ;
  rdfs:subClassOf sosa-core:Observer ;
.
sosa-core:featureOfInterest
  rdf:type owl:ObjectProperty ;
  schema:domainIncludes sosa-core:Observation ;
  schema:rangeIncludes owl:Thing ;
  rdfs:comment "A relation between an Observation and the entity whose quality was observed. For example, in an Observation of the weight of a person, the feature of interest is the person and the quality is weight."^^xsd:string ;
  rdfs:label "feature of interest"@en ;
.
sosa-core:hasResult
  rdf:type owl:ObjectProperty ;
  schema:domainIncludes sosa-core:Observation ;
  schema:domainIncludes sosa-core:Procedure ;
  rdfs:comment "Relation linking an Observation and a Sensor or Actuator and a Result, which contains a value representing the value associated with the observed Property."^^xsd:string ;
  rdfs:label "result"@en ;
.
sosa-core:hostedBy
  rdf:type owl:ObjectProperty ;
  schema:domainIncludes sosa-core:Device ;
  schema:rangeIncludes sosa-core:Platform ;
  rdfs:comment "Relation between a Device and the Platform that it is mounted on or hosted by."^^xsd:string ;
  rdfs:label "hosted by"^^xsd:string ;
.
sosa-core:hosts
  rdf:type owl:ObjectProperty ;
  schema:domainIncludes sosa-core:Platform ;
  schema:rangeIncludes sosa-core:Device ;
  rdfs:comment "Relation between a Platform and a Device hosted or mounted on it."^^xsd:string ;
  rdfs:label "hosts"^^xsd:string ;
.
sosa-core:madeObservation
  rdf:type owl:ObjectProperty ;
  schema:domainIncludes sosa-core:SensingProcedure ;
  schema:rangeIncludes sosa-core:Observation ;
  rdfs:comment "Relation between a Sensor and an Observations it has made."^^xsd:string ;
  rdfs:label "made observation" ;
.
sosa-core:observedProperty
  rdf:type owl:ObjectProperty ;
  schema:domainIncludes sosa-core:Observation ;
  schema:rangeIncludes sosa-core:ObservableProperty ;
  rdfs:comment "Relation linking an Observation to the Property that was observed.  The observedProperty should be a Property (hasProperty) of the FeatureOfInterest (linked by featureOfInterest) of this observation." ;
  rdfs:label "observed property"@en ;
.
sosa-core:observes
  rdf:type owl:ObjectProperty ;
  schema:domainIncludes sosa-core:SensingProcedure ;
  schema:rangeIncludes sosa-core:ObservableProperty ;
  rdfs:comment "Relation between a SensingProcedure and an ObservableProperty."^^xsd:string ;
  rdfs:label "observes"^^xsd:string ;
.
sosa-core:phenomenonTime
  rdf:type owl:ObjectProperty ;
  schema:domainIncludes sosa-core:Observation ;
  rdfs:comment "The time that the Result of an Observation applies to the FeatureOfInterest - not necessarily the same as the result-time."^^xsd:string ;
  rdfs:label "phenomenon time" ;
.
sosa-core:resultTime
  rdf:type owl:DatatypeProperty ;
  schema:domainIncludes sosa-core:Observation ;
  rdfs:comment "The result time is the time when the Procedure associated with the Observation act was completed."^^xsd:string ;
  rdfs:range xsd:dateTime ;
.
sosa-core:sampledFeature
  rdf:type owl:ObjectProperty ;
  schema:domainIncludes sosa-core:SamplingFeature ;
  schema:rangeIncludes owl:Thing ;
  rdfs:comment "Relation from a SamplingFeature to the Feature that it is intended to be representative of." ;
  rdfs:label "sampled feature" ;
.
sosa-core:samplingStrategy
  rdf:type owl:ObjectProperty ;
  schema:domainIncludes sosa-core:Observation ;
  schema:rangeIncludes sosa-core:SamplingFeature ;
  schema:rangeIncludes sosa-core:SamplingProcedure ;
  rdfs:comment "Relation from an Observation or Sensing activity to a SamplingFeature or SamplingProcedure."@en ;
  rdfs:label "sampling strategy"@en ;
.
sosa-core:usedProcedure
  rdf:type owl:ObjectProperty ;
  schema:domainIncludes sosa-core:Observation ;
  schema:rangeIncludes sosa-core:Procedure ;
  rdfs:comment "Link to a re-usable Procedure used in making Observation. Typically a sensor or sensor-system, algorithm, computational procedure."^^xsd:string ;
  rdfs:label "observation procedure"@en ;
.
