# baseURI: https://www.w3.org/ns/sosa
# imports: http://schema.org

@prefix dc: <http://purl.org/dc/elements/1.1/> .
@prefix meta: <http://meta.schema.org/> .
@prefix ns: <http://creativecommons.org/ns#> .
@prefix owl: <http://www.w3.org/2002/07/owl#> .
@prefix rdf: <http://www.w3.org/1999/02/22-rdf-syntax-ns#> .
@prefix rdfs: <http://www.w3.org/2000/01/rdf-schema#> .
@prefix schema: <http://schema.org/> .
@prefix sosa-core: <https://www.w3.org/ns/sosa#> .
@prefix terms: <http://purl.org/dc/terms/> .
@prefix xhtm: <http://www.w3.org/1999/xhtml> .
@prefix xsd: <http://www.w3.org/2001/XMLSchema#> .

ns:license
  rdf:type owl:AnnotationProperty ;
.
meta:domainIncludes
  rdf:type owl:AnnotationProperty ;
.
meta:rangeIncludes
  rdf:type owl:AnnotationProperty ;
.
dc:creator
  rdf:type owl:AnnotationProperty ;
.
dc:date
  rdf:type owl:AnnotationProperty ;
.
dc:identifier
  rdf:type owl:AnnotationProperty ;
.
dc:rights
  rdf:type owl:AnnotationProperty ;
.
dc:source
  rdf:type owl:AnnotationProperty ;
.
dc:title
  rdf:type owl:AnnotationProperty ;
.
terms:created
  rdf:type owl:AnnotationProperty ;
.
terms:modified
  rdf:type owl:AnnotationProperty ;
.
rdfs:comment
  rdf:type owl:AnnotationProperty ;
.
rdfs:isDefinedBy
  rdf:type owl:AnnotationProperty ;
.
rdfs:label
  rdf:type owl:AnnotationProperty ;
.
rdfs:seeAlso
  rdf:type owl:AnnotationProperty ;
.
owl:topObjectProperty
  rdf:type owl:ObjectProperty ;
.
<https://www.w3.org/ns/sosa>
  rdf:type owl:Ontology ;
  rdfs:comment "Sensing, Observing, Sampling, and Actuating (SOSA) Core Ontology "^^xsd:string ;
  rdfs:comment "This ontology is based on the SSN Ontology by the W3C Semantic Sensor Networks Incubator Group (SSN-XG), together with considerations from the W3C/OGC Spatial Data on the Web Working Group."^^xsd:string ;
  rdfs:comment "This version is based on the horizontal/vertical modularization proposed by Jano for the W3C/OGC Spatial Data on the Web Working Group: https://www.w3.org/2015/spatial/wiki/SOSA_Ontology and https://www.w3.org/2015/spatial/wiki/SSN_core_modules"^^xsd:string ;
  rdfs:label "Sensing, Observing, Sampling, and Actuating"^^xsd:string ;
  owl:imports <http://schema.org> ;
.
sosa-core:Actuation
  rdf:type owl:Class ;
  rdfs:comment "An Actuation carries out an (actuation) Procedure to change the state of the world via an Actuator."@en ;
  rdfs:label "Actuation"@en ;
.
sosa-core:Actuator
  rdf:type owl:Class ;
  rdfs:comment "A device that is used by, or implements, an (actuating) Procedure."@en ;
  rdfs:label "Actuator"@en ;
.
sosa-core:FeatureOfInterest
  rdf:type owl:Class ;
  rdfs:comment "The feature whose ObservableProperty is being observed by a Sensor to arrive at a Result. For example, when measuring the height of a tree, said height is the ObservedProperty, 20m may be the Result of the Observation, and the tree is the FeatureOfInterest. "@en ;
  rdfs:label "Feature Of Interest"@en ;
.
sosa-core:Host
  rdf:type owl:Class ;
  rdfs:comment "A device, system, platform, or agent (including humans). a host carries at least one Sensor or Actuator (or Sampling-Device) to produce observations or actuations or samples, by following a Procedure."@en ;
  rdfs:label "Host"@en ;
.
sosa-core:ObservableProperty
  rdf:type owl:Class ;
  rdfs:comment "An observable Quality of a thing; typically a FeatureOfInterest."@en ;
  rdfs:label "Observable Property"@en ;
.
sosa-core:Observation
  rdf:type owl:Class ;
  rdfs:comment "An Observation carries out an (observation) Procedure to estimate or calculate a value of a Property of a FeatureOfInterest. Links to an Host or Sensor to describe what made the Observation and how; links to an ObservableProperty to describe what the result is an estimate of, and to a FeatureOfInterest to detail what that property was associated with; the Result is the output."@en ;
  rdfs:label "Observation"@en ;
.
sosa-core:Procedure
  rdf:type owl:Class ;
  rdfs:comment "A workflow, protocol, plan, algorithm, or computational method specifying how to set up an Observation, take a Sample, or make a change to the state of the world (via an Actuator). A Procedure is re-usable, and might be involved in many observations, samplings, or actuations. It explains the steps to be carried out to arrive at reproducible results. Put differently, millions of observations may be created via the same Procedure the same way as millions of tables are assembled using the same instructions (as information objects, not their concrete realization). "@en ;
  rdfs:label "Procedure"@en ;
.
sosa-core:Result
  rdf:type owl:Class ;
  rdfs:comment "The result of an observation or actuation, e.g., the value for on observed property of some feature of interest such as 20m for the height of a tree."@en ;
  rdfs:label "Result"@en ;
.
sosa-core:Sample
  rdf:type owl:Class ;
  rdfs:comment "Feature on which observations may be made, which is intended to be representative of a FeatureOfInterest that is not fully accessible."@en ;
  rdfs:comment """Samples are artifacts of an observational strategy, and have no significant function outside of their role in the observation process. The physical characteristics of the features themselves are of little interest, except perhaps to the manager of a sampling campaign.

EXAMPLE A “station” is essentially an identifiable locality where a sensor system or procedure may be deployed and an observation made. In the context of the observation model, it connotes the “world in the vicinity of the station”, so the observed properties relate to the physical medium at the station, and not to any physical artifact such as a mooring, buoy, benchmark, monument, well, etc.

NOTE A transient sample, such as a ships-track or flight-line, might be identified and described, but is unlikely to be revisited exactly.

A sample is intended to sample some feature-of-interest in an application domain, so there is an expectation of at least one sampledFeature property. However, in some cases the identity, and even the exact type, of the sampled feature may not be known when observations are made using the sampling features."""@en ;
  rdfs:label "Sample"@en ;
.
sosa-core:Sensor
  rdf:type owl:Class ;
  rdfs:comment "Device or agent involved in, or implementing, a (sensing) Procedure. Sensors responds to a stimulus, e.g., a change in the environment, and generates a result. Sensors can be mounted on observers, e.g., a modern smart phone hosts multiple sensors."@en ;
  rdfs:comment "Does this also include (something) that implements an interpretation procedures?"^^xsd:string ;
  rdfs:comment "Does this also include software used to implement a simulation or forecasting procedures?"^^xsd:string ;
  rdfs:label "Sensor"@en ;
.
sosa-core:featureOfInterest
  rdf:type owl:ObjectProperty ;
  meta:domainIncludes sosa-core:Observation ;
  meta:rangeIncludes sosa-core:FeatureOfInterest ;
  rdfs:comment "A relation between an Observation and the entity whose quality was observed. For example, in an Observation of the weight of a person, the feature of interest is the person and the quality is weight."^^xsd:string ;
  rdfs:label "feature of interest"@en ;
.
sosa-core:hasResult
  rdf:type owl:ObjectProperty ;
  meta:domainIncludes sosa-core:Observation ;
  meta:domainIncludes sosa-core:Result ;
  rdfs:comment "Relation linking an Observation and a Sensor or Actuator and a Result, which contains a value representing the value associated with the observed Property."^^xsd:string ;
  rdfs:label "result"@en ;
.
sosa-core:hostedBy
  rdf:type owl:ObjectProperty ;
  meta:domainIncludes sosa-core:Actuator ;
  meta:domainIncludes sosa-core:Sensor ;
  meta:rangeIncludes sosa-core:Host ;
  rdfs:comment "Relation between a Sensor or Actuator and the Host that it is mounted on or hosted by."^^xsd:string ;
  rdfs:label "hosted by"^^xsd:string ;
.
sosa-core:hosts
  rdf:type owl:ObjectProperty ;
  meta:domainIncludes sosa-core:Host ;
  meta:rangeIncludes sosa-core:Actuator ;
  meta:rangeIncludes sosa-core:Sensor ;
  rdfs:comment "Relation between a Host and a Sensor or Actuator (or SamplingDevice) hosted or mounted on it."^^xsd:string ;
  rdfs:label "hosts"^^xsd:string ;
.
sosa-core:madeObservation
  rdf:type owl:ObjectProperty ;
  meta:domainIncludes sosa-core:Sensor ;
  meta:rangeIncludes sosa-core:Observation ;
  rdfs:comment "Relation between a Sensor and an Observations it has made."^^xsd:string ;
  rdfs:label "made observation" ;
.
sosa-core:observedProperty
  rdf:type owl:ObjectProperty ;
  meta:domainIncludes sosa-core:Observation ;
  meta:rangeIncludes sosa-core:ObservableProperty ;
  rdfs:comment "Relation linking an Observation to the Property that was observed.  The observedProperty should be a Property (hasProperty) of the FeatureOfInterest (linked by featureOfInterest) of this observation." ;
  rdfs:label "observed property"@en ;
.
sosa-core:observes
  rdf:type owl:ObjectProperty ;
  meta:domainIncludes sosa-core:Sensor ;
  meta:rangeIncludes sosa-core:ObservableProperty ;
  rdfs:comment "Relation between a Sensor and an ObservableProperty."^^xsd:string ;
  rdfs:label "observes"^^xsd:string ;
.
sosa-core:phenomenonTime
  rdf:type owl:ObjectProperty ;
  meta:domainIncludes sosa-core:Actuation ;
  meta:domainIncludes sosa-core:Observation ;
  rdfs:comment "The time that the Result of an Observation/Actuation applies to the FeatureOfInterest - not necessarily the same as the result-time."^^xsd:string ;
  rdfs:label "phenomenon time" ;
.
sosa-core:resultTime
  rdf:type owl:DatatypeProperty ;
  meta:domainIncludes sosa-core:Actuation ;
  meta:domainIncludes sosa-core:Observation ;
  rdfs:comment "The result time is the time when the Observation/Actuation act was completed."^^xsd:string ;
  rdfs:range xsd:dateTime ;
.
sosa-core:sampledFeature
  rdf:type owl:ObjectProperty ;
  meta:domainIncludes sosa-core:Sample ;
  rdfs:comment "Relation from a Sample to the FeatureOfInterest that it is intended to be representative of." ;
  rdfs:label "sampled feature" ;
.
sosa-core:usedProcedure
  rdf:type owl:ObjectProperty ;
  meta:domainIncludes sosa-core:Actuation ;
  meta:domainIncludes sosa-core:Observation ;
  meta:rangeIncludes sosa-core:Procedure ;
  rdfs:comment "Link to a re-usable Procedure used in making Observation or Actuation. Typically a sensor or sensor-system, algorithm, computational procedure."^^xsd:string ;
  rdfs:label "observation procedure"@en ;
.
