# baseURI: http://www.w3.org/ns/sosa-oml
# imports: http://def.seegrid.csiro.au/ontology/om/om-lite
# imports: http://def.seegrid.csiro.au/ontology/om/sam-lite
# imports: http://www.w3.org/ns/sosa/

@prefix dc: <http://purl.org/dc/elements/1.1/> .
@prefix dcterms: <http://purl.org/dc/terms/> .
@prefix oml: <http://def.seegrid.csiro.au/ontology/om/om-lite#> .
@prefix owl: <http://www.w3.org/2002/07/owl#> .
@prefix rdf: <http://www.w3.org/1999/02/22-rdf-syntax-ns#> .
@prefix rdfs: <http://www.w3.org/2000/01/rdf-schema#> .
@prefix samfl: <http://def.seegrid.csiro.au/ontology/om/sam-lite#> .
@prefix sosa: <http://www.w3.org/ns/sosa/> .
@prefix xsd: <http://www.w3.org/2001/XMLSchema#> .

oml:Observation
  owl:equivalentClass sosa:Observation ;
.
oml:Process
  rdfs:subClassOf [
      rdf:type owl:Class ;
      owl:unionOf (
          sosa:Procedure
          sosa:Sensor
        ) ;
    ] ;
.
oml:featureOfInterest
  owl:equivalentProperty sosa:hasFeatureOfInterest ;
.
oml:observedProperty
  owl:equivalentProperty sosa:observedProperty ;
.
oml:phenomenonTime
  owl:equivalentProperty sosa:phenomenonTime ;
.
oml:procedure
  rdfs:comment "sub-property of sosa:usedPropecedure which also covers procedures for actuation and sampling" ;
  rdfs:subPropertyOf sosa:usedProcedure ;
.
oml:result
  rdfs:comment "sub-property of sosa:hasResult which also covers actuation and sampling" ;
  rdfs:subPropertyOf sosa:hasResult ;
.
oml:resultTime
  rdfs:comment "sub-property of sosa:resultTime which also relates to actuation and sampling events" ;
  rdfs:subPropertyOf sosa:resultTime ;
.
samfl:Process
  rdfs:subClassOf [
      rdf:type owl:Class ;
      owl:unionOf (
          sosa:Procedure
          <http://www.w3.org/ns/sosa-oml/SamplingDevice>
        ) ;
    ] ;
.
samfl:SamplingFeature
  owl:equivalentClass sosa:Sample ;
.
samfl:hostedProcedure
  rdfs:comment "When a sampling feature hosts a procedure or instrument it is acting as a platform." ;
  rdfs:comment "sub-property of sosa:hosts which relates a platform to an observation, actuation or sampling procedure" ;
  rdfs:subPropertyOf sosa:hosts ;
.
samfl:sampledFeature
  owl:equivalentProperty sosa:isSampleOf ;
.
samfl:samplingTime
  rdfs:comment "sub-property of sosa:resultTime which also relates to actuation and observation events" ;
  rdfs:subPropertyOf sosa:resultTime ;
.
<http://www.w3.org/ns/sosa-oml>
  rdf:type owl:Ontology ;
  dc:creator "Simon J D Cox" ;
  dcterms:created "2016-12-14" ;
  rdfs:comment """Mapping of the om-lite/sam-lite implementations of O&M with the W3C/OGC SOSA ontology. 

N.B. om-lite/sam-lite are idiomatic OWL implementations of the O&M model from ISO 19156:2011, 
documented in Semantic Web Journal, v8, n3 2017"""@en ;
  rdfs:label "Alignment of om-lite + sam-lite with SOSA"@en ;
  owl:imports <http://def.seegrid.csiro.au/ontology/om/om-lite> ;
  owl:imports <http://def.seegrid.csiro.au/ontology/om/sam-lite> ;
  owl:imports sosa: ;
.
<http://www.w3.org/ns/sosa-oml#SamplingDevice>
  rdf:type owl:Class ;
  rdfs:comment "Notional superclass of all devices that implement sampling procedures." ;
  rdfs:label "Sampling or sample processing device" ;
.
sosa:Observation
  owl:equivalentClass oml:Observation ;
.
sosa:Sample
  owl:equivalentClass samfl:SamplingFeature ;
.
sosa:Sensor
  rdfs:subClassOf oml:Process ;
.
sosa:hasFeatureOfInterest
  owl:equivalentProperty oml:featureOfInterest ;
.
sosa:isSampleOf
  owl:equivalentProperty samfl:sampledFeature ;
.
sosa:observedProperty
  owl:equivalentProperty oml:observedProperty ;
.
sosa:phenomenonTime
  owl:equivalentProperty oml:phenomenonTime ;
.
